adder: specification for the full setup

theories/examples/adder.v
@@ -312,4 +312,194 @@ Section adder.
     auto.
   Qed.
 
+
+  (* "full system" specification, starting from the execution of [g] *)
+
+  Definition closureN : namespace := nroot .@ "adder" .@ "closure".
+  Definition actN : namespace := nroot .@ "adder" .@ "act".
+
+  Lemma adder_full_spec af ag g_start x x' w0 w2 act0 rmap act_start act_end :
+    contiguous_between ag g_start f_start →
+    contiguous_between af f_start f_end →
+    (x+1)%a = Some x' →
+    (act_start + 8)%a = Some act_end →
+    (f_start <= f_end)%a →
+    dom (gset RegName) rmap = all_registers_s ∖ {[ PC; r_t0; r_t1; r_t2; r_t3 ]} →
+
+    inv N (∃ (n:Z), x ↦ₐ inl n ∗ ⌜(0 ≤ n)%Z⌝)
+    ∗ adder_g ag ∗ adder_f af
+    ∗ PC ↦ᵣ inr (RX, g_start, f_end, g_start)
+    ∗ r_t0 ↦ᵣ w0
+    ∗ r_t1 ↦ᵣ inr (RWX, act_start, act_end, act_start)
+    ∗ r_t2 ↦ᵣ w2
+    ∗ r_t3 ↦ᵣ inr (RW, x, x', x)
+    ∗ [[act_start, act_end]] ↦ₐ [[ act0 ]]
+    ∗ interp w0
+    ∗ ([∗ map] r↦v ∈ rmap, r ↦ᵣ v ∗ interp v)
+    ∗ na_own logrel_nais ⊤
+    -∗ WP Seq (Instr Executable) {{ λ _, True }}.
+  Proof.
+    iIntros (Hcontg Hcontf Hx' Hact_start_end Hf_start_end Hrmap_dom)
+            "(#Hinv & Hprog_g & Hprog_f & HPC & Hr0 & Hr1 & Hr2 & Hr3 & Hact & #Hw0 & Hregs & HnaI)".
+    iApply (wp_wand with "[-]"). 2: iIntros (?) "_"; eauto.
+    (* Step 1: Use the spec for g *)
+    iApply (adder_g_spec with "[- $HPC $Hr0 $Hr1 $Hr2 $Hr3 $Hact $Hprog_g]"); auto.
+    (* Step 2: Use the validity of w0 and the FTLR *)
+    iPoseProof (jmp_or_fail_spec _ (λ _, True)%I with "Hw0") as "Hcont".
+    destruct (decide (isCorrectPC (updatePcPerm w0))); cycle 1.
+    { (* the jump might fail: that's OK. *)
+      iNext. iIntros "(? & ? & ? & ? & ? & ?)".
+      iApply "Hcont". iFrame. }
+    (* otherwise, we get that the continuation satisfies the expression relation *)
+    iDestruct "Hcont" as (p b e a ->) "#Ew0". iNext.
+    iIntros "(HPC & Hprog_g & Hr0 & Hr1 & Hr2 & Hr3 & Hact)".
+
+    (* Step 3: Prove that the closure is valid, by using the spec of [f] *)
+    (* Put the code of [f] and the activation record in invariants *)
+    iDestruct (na_inv_alloc logrel_nais _ closureN with "Hprog_f") as ">#Iprog_f".
+    iDestruct (na_inv_alloc logrel_nais _ actN with "Hact") as ">#Iact".
+
+    iAssert (interp (inr (E, act_start, act_end, act_start))) with "[Iprog_f Iact]"
+      as "Hclosure".
+    { iClear "Ew0 Hw0". rewrite /interp /= fixpoint_interp1_eq /=.
+      iIntros (rmap'). iNext. iAlways. iIntros "([Hrmap' #HrV] & Hregs & HnaI)".
+      iDestruct "Hrmap'" as %Hrmap'. iSplit; eauto. rewrite /interp_conf.
+      (* extract registers relevant for f from the map *)
+      iDestruct (big_sepM_delete _ _ PC with "Hregs") as "[HPC Hregs]".
+      by rewrite lookup_insert.
+      destruct (Hrmap' r_t0) as [rv0 Hrv0].
+      iDestruct (big_sepM_delete _ _ r_t0 with "Hregs") as "[Hr0 Hregs]".
+      by rewrite lookup_delete_ne // lookup_insert_ne //.
+      destruct (Hrmap' r_t1) as [rv1 Hrv1].
+      iDestruct (big_sepM_delete _ _ r_t1 with "Hregs") as "[Hr1 Hregs]".
+      by rewrite !lookup_delete_ne // lookup_insert_ne //.
+      destruct (Hrmap' r_t2) as [rv2 Hrv2].
+      iDestruct (big_sepM_delete _ _ r_t2 with "Hregs") as "[Hr2 Hregs]".
+      by rewrite !lookup_delete_ne // lookup_insert_ne //.
+      destruct (Hrmap' r_t3) as [rv3 Hrv3].
+      iDestruct (big_sepM_delete _ _ r_t3 with "Hregs") as "[Hr3 Hregs]".
+      by rewrite !lookup_delete_ne // lookup_insert_ne //.
+      destruct (Hrmap' r_env) as [rvenv Hrvenv].
+      iDestruct (big_sepM_delete _ _ r_env with "Hregs") as "[Hrenv Hregs]".
+      by rewrite !lookup_delete_ne // lookup_insert_ne //.
+      (* Access the activation record code by opening the corresponding invariant;
+         then use the spec for the activation record *)
+      iDestruct (na_inv_open with "Iact HnaI") as ">(>Hact & HnaI & Hact_close)";
+        [auto..|].
+      iApply (closure_activation_spec with "[- $HPC $Hr1 $Hrenv $Hact]"); auto.
+      { intros ? ?. constructor; auto. }
+      iIntros "(HPC & Hr1 & Hrenv & Hact)".
+      iDestruct ("Hact_close" with "[$HnaI $Hact]") as ">HnaI". (* close the invariant *)
+      (* Now, access the code of f and use its specification *)
+      iDestruct (na_inv_open with "Iprog_f HnaI") as ">(>Hprog_f & HnaI & Hprog_f_close)";
+        [auto..|].
+      iApply (wp_wand with "[-]").
+      { iApply (adder_f_spec with "[- $HPC $Hr0 $Hr1 $Hr2 $Hr3 $Hrenv $Hprog_f]"); auto.
+        iSplitL "Hinv"; eauto.
+        (* Use the fact that the closure's continuation is valid to conclude *)
+        (* This involves a lot of bureaucratic shuffling of the register resources *)
+        unshelve iPoseProof ("HrV" $! r_t0 _) as "Hr0V";[done|].
+        rewrite /RegLocate Hrv0.
+        pose (λ v, ⌜v = HaltedV⌝ → ∃ r, full_map r ∧ registers_mapsto r ∗ na_own logrel_nais ⊤)%I as φ.
+        iPoseProof (jmp_or_fail_spec _ φ with "Hr0V") as "Hcont".
+        destruct (decide (isCorrectPC (updatePcPerm rv0))); cycle 1.
+        { iNext. iIntros "H". iApply "Hcont". iDestruct "H" as (? ?) "(? & ?)". iFrame.
+          rewrite /φ /=. iIntros (?). congruence. }
+        iDestruct "Hcont" as (p' b' e' a' ->) "Hcont". iNext.
+        iIntros "HH". iDestruct "HH" as (k' n') "(HPC & Hprog_f & Hr0 & Hr1 & Hr2 & Hr3 & Hrenv)".
+        iDestruct ("Hprog_f_close" with "[$HnaI $Hprog_f]") as ">HnaI". (* close *)
+        (* Put the registers back in the map *)
+        iDestruct (big_sepM_insert with "[$Hregs $Hr0]") as "Hregs".
+        by repeat (rewrite lookup_delete_ne //;[]); rewrite lookup_delete //.
+        repeat (rewrite -delete_insert_ne //;[]). rewrite insert_delete.
+        iDestruct (big_sepM_insert with "[$Hregs $Hr1]") as "Hregs".
+        by repeat (rewrite lookup_delete_ne //;[]); rewrite lookup_delete //.
+        repeat (rewrite -delete_insert_ne //;[]). rewrite insert_delete.
+        iDestruct (big_sepM_insert with "[$Hregs $Hr2]") as "Hregs".
+        by repeat (rewrite lookup_delete_ne //;[]); rewrite lookup_delete //.
+        repeat (rewrite -delete_insert_ne //;[]). rewrite insert_delete.
+        iDestruct (big_sepM_insert with "[$Hregs $Hr3]") as "Hregs".
+        by repeat (rewrite lookup_delete_ne //;[]); rewrite lookup_delete //.
+        repeat (rewrite -delete_insert_ne //;[]). rewrite insert_delete.
+        iDestruct (big_sepM_insert with "[$Hregs $Hrenv]") as "Hregs".
+        by repeat (rewrite lookup_delete_ne //;[]); rewrite lookup_delete //.
+        repeat (rewrite -delete_insert_ne //;[]). rewrite insert_delete.
+        iDestruct (big_sepM_insert with "[$Hregs $HPC]") as "Hregs".
+        rewrite !lookup_insert_ne // lookup_delete //.
+        match goal with |- context [ ([∗ map] _↦_ ∈ ?r, _)%I ] => set rmap'' := r end.
+        iAssert (full_map rmap'') as %Hrmap''_full.
+        { rewrite /full_map. iIntros (rr). iPureIntro. rewrite elem_of_gmap_dom /rmap''.
+          rewrite !dom_insert_L !dom_delete_L !dom_insert_L regmap_full_dom //.
+          rewrite !singleton_union_difference_L !all_registers_union_l.
+          pose proof (all_registers_s_correct rr) as HH. set_solver+ HH. }
+
+        iSpecialize ("Hcont" $! rmap'' with "[Hregs HnaI]").
+        { iFrame. iSplitR.
+          { rewrite /interp_reg /=. iSplit; auto. iIntros (r Hr).
+            specialize (Hrmap''_full r) as [rv Hrv]. rewrite /RegLocate Hrv.
+            unshelve iSpecialize ("HrV" $! r _); auto.
+            rewrite /rmap'' in Hrv. rewrite (fixpoint_interp1_eq rv).
+            destruct (decide (r = r_env)); subst.
+            { rewrite lookup_insert_ne // lookup_insert in Hrv. by simplify_eq. }
+            destruct (decide (r = r_t3)); subst.
+            { repeat (rewrite lookup_insert_ne // in Hrv;[]); rewrite lookup_insert // in Hrv.
+              by simplify_eq. }
+            destruct (decide (r = r_t2)); subst.
+            { repeat (rewrite lookup_insert_ne // in Hrv;[]); rewrite lookup_insert // in Hrv.
+              by simplify_eq. }
+            destruct (decide (r = r_t1)); subst.
+            { repeat (rewrite lookup_insert_ne // in Hrv;[]); rewrite lookup_insert // in Hrv.
+              by simplify_eq. }
+            destruct (decide (r = r_t0)); subst.
+            { repeat (rewrite lookup_insert_ne // in Hrv;[]); rewrite lookup_insert // in Hrv.
+              simplify_eq. rewrite !fixpoint_interp1_eq //. }
+            repeat (rewrite lookup_insert_ne // in Hrv;[]).
+            rewrite delete_insert_delete lookup_delete_ne // in Hrv.
+            rewrite Hrv !fixpoint_interp1_eq //. }
+          { rewrite /registers_mapsto /rmap'' insert_insert //. } }
+
+        iDestruct "Hcont" as "[_ Hcont]". rewrite /interp_conf.
+        iApply (wp_wand with "[-]"). iApply "Hcont". cbn. iIntros (v) "?". eauto.
+      }
+      { cbn. iIntros (?) "[H|%]"; iIntros (->). iApply "H"; eauto. congruence. }
+    }
+
+    (* Step 4: use the fact that the continuation is in the expression relation *)
+    (* put the registers back in the map *)
+    iDestruct (big_sepM_insert with "[$Hregs $Hr3]") as "Hregs".
+    { apply elem_of_gmap_dom_none. set_solver+ Hrmap_dom. }
+    { rewrite /interp /= !fixpoint_interp1_eq //. }
+    iDestruct (big_sepM_insert with "[$Hregs $Hr2]") as "Hregs".
+    { rewrite lookup_insert_ne //. apply elem_of_gmap_dom_none. set_solver+ Hrmap_dom. }
+    { rewrite /interp /= !fixpoint_interp1_eq //. }
+    iDestruct (big_sepM_insert with "[$Hregs $Hr1 Hclosure]") as "Hregs".
+    { rewrite !lookup_insert_ne //. apply elem_of_gmap_dom_none. set_solver+ Hrmap_dom. }
+    { eauto. }
+    iDestruct (big_sepM_insert with "[$Hregs $Hr0]") as "Hregs".
+    { rewrite !lookup_insert_ne //. apply elem_of_gmap_dom_none. set_solver+ Hrmap_dom. }
+    { eauto. }
+    match goal with |- context [ ([∗ map] _↦_ ∈ ?r, _)%I ] => set rmap' := r end.
+    iDestruct (big_sepM_sep with "Hregs") as "[Hregs HregsV]".
+    iDestruct (big_sepM_insert with "[$Hregs $HPC]") as "Hregs".
+    { rewrite !lookup_insert_ne //. apply elem_of_gmap_dom_none. set_solver+ Hrmap_dom. }
+    set rmap'' := <[_:=_]> rmap'.
+    iAssert (full_map rmap'') as %Hrmap''_full.
+    { rewrite /full_map. iIntros (rr). iPureIntro. rewrite elem_of_gmap_dom /rmap'' /rmap'.
+      rewrite !dom_insert_L Hrmap_dom.
+      rewrite !singleton_union_difference_L !all_registers_union_l.
+      pose proof (all_registers_s_correct rr) as H. set_solver+ H. }
+
+    iSpecialize ("Ew0" $! rmap'' with "[Hregs HregsV HnaI]").
+    { iFrame. iSplitR "Hregs"; cycle 1.
+      { rewrite /registers_mapsto /rmap'' insert_insert. eauto. }
+      rewrite /interp_reg /=. iSplit; eauto. iIntros (r Hr).
+      destruct (Hrmap''_full r) as [rv Hrv].
+      iDestruct (big_sepM_lookup _ _ r with "HregsV") as "Hr"; eauto.
+      rewrite /rmap'' /RegLocate (lookup_insert_ne _ PC) // in Hrv |- *.
+      rewrite Hrv //. }
+
+    iDestruct "Ew0" as "[_ Hcont]". iApply (wp_wand with "[-]"). iApply "Hcont".
+    eauto.
+  Qed.
+
 End adder.
